sync

coq/SimpleForm/Simplifications/ReplaceVar.v
@@ -39,18 +39,19 @@ Section ReplaceVar.
   Definition replace_var (sf: simple_form) (from: positive) (to: sact)
   : simple_form := {|
     final_values := final_values sf;
-    vars := replace_var_in_vars (vars sf) from to; |}.
-
+    vars := replace_var_in_vars (vars sf) from to
+  |}.
 
   Lemma wt_sact_replace_var_in_vars:
     forall vvs a i v t tv,
-      wt_sact (Sigma:=Sigma) R vvs a t
-      -> wt_sact (Sigma:=Sigma) R vvs (SVar i) tv
-      -> wt_sact (Sigma:=Sigma) R vvs v tv
-      -> wt_sact (Sigma:=Sigma) R (replace_var_in_vars vvs i v) a t.
+    wt_sact (Sigma:=Sigma) R vvs a t
+    -> wt_sact (Sigma:=Sigma) R vvs (SVar i) tv
+    -> wt_sact (Sigma:=Sigma) R vvs v tv
+    -> wt_sact (Sigma:=Sigma) R (replace_var_in_vars vvs i v) a t.
   Proof.
     induction a; simpl; intros; eauto.
-    inv H. inv H0. econstructor; eauto. setoid_rewrite PTree.gmap. setoid_rewrite H3.
+    inv H. inv H0. econstructor; eauto. setoid_rewrite PTree.gmap.
+    setoid_rewrite H3.
     simpl; eauto.
     inv H; econstructor; eauto.
     inv H; econstructor; eauto.
@@ -61,24 +62,20 @@ Section ReplaceVar.
   Qed.
 
   Lemma interp_sact_replace_var:
-    forall vvs
-           (WTvvs: wt_vvs R (Sigma:=Sigma) vvs)
-           (VSV: vvs_smaller_variables vvs)
-           idx v
-           (SAME1: forall ov,
-               interp_sact (sigma:=sigma) REnv r vvs (SVar idx) ov <->
-                 interp_sact (sigma:=sigma) REnv r vvs v ov
-           )
-           (SMALLER: forall var, reachable_var vvs v var -> (var < idx)%positive)
-           (tt : type)
-           (OLDTYPE : wt_sact R (Sigma:=Sigma) vvs (SVar idx) tt)
-           (NEWTYPE : wt_sact R (Sigma:=Sigma) vvs v tt)
-           a n (LT: forall v, reachable_var vvs a v -> (v < n)%positive)
-           t
-           (WT: wt_sact (Sigma:=Sigma) R vvs a t),
+    forall
+      vvs (WTvvs: wt_vvs R (Sigma:=Sigma) vvs) (VSV: vvs_smaller_variables vvs)
+      idx v
+      (SAME1: forall ov,
+       interp_sact (sigma:=sigma) REnv r vvs (SVar idx) ov
+       <-> interp_sact (sigma:=sigma) REnv r vvs v ov)
+      (SMALLER: forall var, reachable_var vvs v var -> (var < idx)%positive)
+      (tt : type) (OLDTYPE: wt_sact R (Sigma:=Sigma) vvs (SVar idx) tt)
+      (NEWTYPE: wt_sact R (Sigma:=Sigma) vvs v tt) a n
+      (LT: forall v, reachable_var vvs a v -> (v < n)%positive) t
+      (WT: wt_sact (Sigma:=Sigma) R vvs a t),
     forall vv,
-      interp_sact (sigma:=sigma) REnv r vvs a vv <->
-        interp_sact (sigma:=sigma) REnv r (replace_var_in_vars vvs idx v) a vv.
+    interp_sact (sigma:=sigma) REnv r vvs a vv
+    <-> interp_sact (sigma:=sigma) REnv r (replace_var_in_vars vvs idx v) a vv.
   Proof.
     intros vvs WTvvs VSV idx v SAME1 SMALLER tt OLDTYPE NEWTYPE a n.
     change n with (projT1 (existT (fun _ => sact) n a)).
@@ -93,12 +90,10 @@ Section ReplaceVar.
         forall a0,
         size_sact a0 < size_sact (projT2 x)
         -> (forall v0, reachable_var vvs a0 v0 -> (v0 < projT1 x)%positive)
-        ->
-          forall t
-                 (WT: wt_sact (Sigma:=Sigma) R vvs a0 t),
-            forall vv,
-      interp_sact (sigma:=sigma) REnv r vvs a0 vv <->
-        interp_sact (sigma:=sigma) REnv r (replace_var_in_vars vvs idx v) a0 vv
+        -> forall t (WT: wt_sact (Sigma:=Sigma) R vvs a0 t), forall vv,
+          interp_sact (sigma:=sigma) REnv r vvs a0 vv
+          <-> interp_sact
+                (sigma:=sigma) REnv r (replace_var_in_vars vvs idx v) a0 vv
     ). {
       intros. eapply (IH (existT _ (projT1 x) a0)).
       red. destruct x. apply Relation_Operators.right_lex. simpl in H.  auto.
@@ -111,19 +106,21 @@ Section ReplaceVar.
       + subst.
         Opaque eq_dec. intros.
         assert (
-            interp_sact (sigma:=sigma) REnv r (replace_var_in_vars vvs var v) (SVar var) vv <->
-                    interp_sact (sigma:=sigma) REnv r (replace_var_in_vars vvs var v) v vv
-          ).
-        {
+          interp_sact
+            (sigma:=sigma) REnv r (replace_var_in_vars vvs var v) (SVar var) vv
+          <-> interp_sact
+                (sigma:=sigma) REnv r (replace_var_in_vars vvs var v) v vv
+        ). {
           split.
           - intro A; inv A.
-            setoid_rewrite PTree.gmap in H1. setoid_rewrite H0 in H1. simpl in H1.
-            destr_in H1; try congruence.
+            setoid_rewrite PTree.gmap in H1. setoid_rewrite H0 in H1.
+            simpl in H1. destr_in H1; try congruence.
           - intro; econstructor; eauto.
             setoid_rewrite PTree.gmap. setoid_rewrite H0. simpl. destr. eauto.
         } rewrite H.
         exploit (IH (existT _ var v)).
-        red. apply Relation_Operators.left_lex. apply BELOW. econstructor. simpl.
+        red. apply Relation_Operators.left_lex. apply BELOW. econstructor.
+        simpl.
         generalize (reachable_var_aux_below_get _ VSV _ _ _ H0). auto. simpl.
         eauto. simpl. intro A; rewrite <- A. apply SAME1.
       + exploit (IH (existT _ var s)).
@@ -132,76 +129,83 @@ Section ReplaceVar.
         generalize (reachable_var_aux_below_get _ VSV _ _ _ H0). auto. simpl.
         eapply WTvvs. eauto. simpl.
         assert (
-            interp_sact (sigma:=sigma) REnv r vvs (SVar var) vv <->
-                    interp_sact (sigma:=sigma) REnv r vvs s vv
-          ).
-        {
-          split. intro A; inv A. congruence. intros; econstructor; eauto.
-        } rewrite H. clear H.
+          interp_sact (sigma:=sigma) REnv r vvs (SVar var) vv
+          <-> interp_sact (sigma:=sigma) REnv r vvs s vv
+        ). { split. intro A; inv A. congruence. intros; econstructor; eauto. }
+        rewrite H. clear H.
         assert (
-            interp_sact (sigma:=sigma) REnv r (replace_var_in_vars vvs idx v) (SVar var) vv <->
-                    interp_sact (sigma:=sigma) REnv r (replace_var_in_vars vvs idx v) s vv
-          ).
-        {
+          interp_sact
+            (sigma:=sigma) REnv r (replace_var_in_vars vvs idx v) (SVar var) vv
+          <-> interp_sact
+                (sigma:=sigma) REnv r (replace_var_in_vars vvs idx v) s vv
+        ). {
           split.
           - intro A; inv A.
-            setoid_rewrite PTree.gmap in H1. setoid_rewrite H0 in H1. simpl in H1.
-            destr_in H1; try congruence.
+            setoid_rewrite PTree.gmap in H1. setoid_rewrite H0 in H1.
+            simpl in H1. destr_in H1; try congruence.
           - intro; econstructor; eauto.
             setoid_rewrite PTree.gmap. setoid_rewrite H0. simpl. destr. eauto.
-        } rewrite H.
-        eauto.
+        }
+        rewrite H. eauto.
     - intros. split; intro A; inv A; econstructor.
     - inv WTs.
       intros.
       split; intro A; inv A.
       + econstructor.
-        eapply (IH2 s1). lia. intros; eapply BELOW. eapply reachable_var_if_cond; eauto. eauto. eauto.
+        eapply (IH2 s1). lia. intros; eapply BELOW.
+        eapply reachable_var_if_cond; eauto. eauto. eauto.
         eapply (IH2 (if b then s2 else s3)).
-        destr; lia. intros; eapply BELOW. destr_in H. eapply reachable_var_if_true; eauto.
+        destr; lia. intros; eapply BELOW. destr_in H.
+        eapply reachable_var_if_true; eauto.
         eapply reachable_var_if_false; eauto.
         destr; eauto. eauto.
       + econstructor.
-        eapply (IH2 s1). lia. intros; eapply BELOW. eapply reachable_var_if_cond; eauto. eauto. eauto.
+        eapply (IH2 s1). lia. intros; eapply BELOW.
+        eapply reachable_var_if_cond; eauto. eauto. eauto.
         eapply (IH2 (if b then s2 else s3)).
-        destr; lia. intros; eapply BELOW. destr_in H. eapply reachable_var_if_true; eauto.
+        destr; lia. intros; eapply BELOW. destr_in H.
+        eapply reachable_var_if_true; eauto.
         eapply reachable_var_if_false; eauto.
         destr; eauto. eauto.
     - inv WTs; intros.
       split; intro A; inv A; econstructor; eauto.
-      eapply (IH2 s). lia. intros; eapply BELOW. eapply reachable_var_unop; eauto. eauto. eauto.
-      eapply (IH2 s). lia. intros; eapply BELOW. eapply reachable_var_unop; eauto. eauto. eauto.
+      eapply (IH2 s). lia. intros; eapply BELOW.
+      eapply reachable_var_unop; eauto. eauto. eauto.
+      eapply (IH2 s). lia. intros; eapply BELOW.
+      eapply reachable_var_unop; eauto. eauto. eauto.
     - inv WTs; intros.
       split; intro A; inv A; econstructor; eauto.
-      eapply (IH2 s1). lia. intros; eapply BELOW. eapply reachable_var_binop1; eauto. eauto. eauto.
-      eapply (IH2 s2). lia. intros; eapply BELOW. eapply reachable_var_binop2; eauto. eauto. eauto.
-      eapply (IH2 s1). lia. intros; eapply BELOW. eapply reachable_var_binop1; eauto. eauto. eauto.
-      eapply (IH2 s2). lia. intros; eapply BELOW. eapply reachable_var_binop2; eauto. eauto. eauto.
+      eapply (IH2 s1). lia. intros; eapply BELOW.
+      eapply reachable_var_binop1; eauto. eauto. eauto.
+      eapply (IH2 s2). lia. intros; eapply BELOW.
+      eapply reachable_var_binop2; eauto. eauto. eauto.
+      eapply (IH2 s1). lia. intros; eapply BELOW.
+      eapply reachable_var_binop1; eauto. eauto. eauto.
+      eapply (IH2 s2). lia. intros; eapply BELOW.
+      eapply reachable_var_binop2; eauto. eauto. eauto.
     - inv WTs; intros.
       split; intro A; inv A; econstructor; eauto.
-      eapply (IH2 s). lia. intros; eapply BELOW. eapply reachable_var_externalCall; eauto. eauto. eauto.
-      eapply (IH2 s). lia. intros; eapply BELOW. eapply reachable_var_externalCall; eauto. eauto. eauto.
+      eapply (IH2 s). lia. intros; eapply BELOW.
+      eapply reachable_var_externalCall; eauto. eauto. eauto.
+      eapply (IH2 s). lia. intros; eapply BELOW.
+      eapply reachable_var_externalCall; eauto. eauto. eauto.
     - intros. split; intro A; inv A; econstructor.
   Qed.
 
   Lemma interp_sact_replace_var':
-    forall vvs
-           (WTvvs: wt_vvs R (Sigma:=Sigma) vvs)
-           (VSV: vvs_smaller_variables vvs)
-           idx v
-           (SAME1: forall ov,
-               interp_sact (sigma:=sigma) REnv r vvs (SVar idx) ov <->
-                 interp_sact (sigma:=sigma) REnv r vvs v ov
-           )
-           (SMALLER: forall var, reachable_var vvs v var -> (var < idx)%positive)
-           (tt : type)
-           (OLDTYPE : wt_sact R (Sigma:=Sigma) vvs (SVar idx) tt)
-           (NEWTYPE : wt_sact R (Sigma:=Sigma) vvs v tt)
-           a t
-           (WT: wt_sact (Sigma:=Sigma) R vvs a t),
+    forall
+      vvs (WTvvs: wt_vvs R (Sigma:=Sigma) vvs) (VSV: vvs_smaller_variables vvs)
+      idx v
+      (SAME1: forall ov,
+       interp_sact (sigma:=sigma) REnv r vvs (SVar idx) ov
+       <-> interp_sact (sigma:=sigma) REnv r vvs v ov)
+      (SMALLER: forall var, reachable_var vvs v var -> (var < idx)%positive)
+      (tt : type) (OLDTYPE: wt_sact R (Sigma:=Sigma) vvs (SVar idx) tt)
+      (NEWTYPE: wt_sact R (Sigma:=Sigma) vvs v tt) a t
+      (WT: wt_sact (Sigma:=Sigma) R vvs a t),
     forall vv,
-      interp_sact (sigma:=sigma) REnv r vvs a vv <->
-        interp_sact (sigma:=sigma) REnv r (replace_var_in_vars vvs idx v) a vv.
+    interp_sact (sigma:=sigma) REnv r vvs a vv
+    <-> interp_sact (sigma:=sigma) REnv r (replace_var_in_vars vvs idx v) a vv.
   Proof.
     intros.
     eapply interp_sact_replace_var; eauto.
@@ -210,10 +214,10 @@ Section ReplaceVar.
   Qed.
 
   Lemma wt_vvs_replace_var_in_vars:
-    forall vvs v reg
-           (WTVVS: wt_vvs (Sigma := Sigma) R vvs)
-           tt (OLDTYPE: wt_sact (Sigma:=Sigma) R vvs (SVar reg) tt)
-           (NEWTYPE: wt_sact (Sigma:=Sigma) R vvs v tt),
+    forall
+      vvs v reg (WTVVS: wt_vvs (Sigma := Sigma) R vvs) tt
+      (OLDTYPE: wt_sact (Sigma:=Sigma) R vvs (SVar reg) tt)
+      (NEWTYPE: wt_sact (Sigma:=Sigma) R vvs v tt),
     wt_vvs (Sigma := Sigma) R (replace_var_in_vars vvs reg v).
   Proof.
     intros. inv OLDTYPE.
@@ -226,10 +230,10 @@ Section ReplaceVar.
   Qed.
 
   Lemma vsv_replace_var_in_vars:
-    forall vvs v reg
-           (VSV: vvs_smaller_variables vvs)
-           (SMALLER: forall var, reachable_var vvs v var -> (var < reg)%positive),
-      vvs_smaller_variables (replace_var_in_vars vvs reg v).
+    forall
+      vvs v reg (VSV: vvs_smaller_variables vvs)
+      (SMALLER: forall var, reachable_var vvs v var -> (var < reg)%positive),
+    vvs_smaller_variables (replace_var_in_vars vvs reg v).
   Proof.
     intros.
     red. intros.
@@ -239,11 +243,12 @@ Section ReplaceVar.
   Qed.
 
   Lemma wf_sf_replace_var':
-    forall reg val sf
-           tt (OLDTYPE: wt_sact (Sigma:=Sigma) R (vars sf) (SVar reg) tt)
-           (NEWTYPE: wt_sact (Sigma:=Sigma) R (vars sf) val tt)
-           (SMALLER:   forall var : positive, reachable_var (vars sf) val var -> (var < reg)%positive),
-      wf_sf sf -> wf_sf (replace_var sf reg val).
+    forall
+      reg val sf tt (OLDTYPE: wt_sact (Sigma:=Sigma) R (vars sf) (SVar reg) tt)
+      (NEWTYPE: wt_sact (Sigma:=Sigma) R (vars sf) val tt)
+      (SMALLER: forall var : positive,
+        reachable_var (vars sf) val var -> (var < reg)%positive),
+    wf_sf sf -> wf_sf (replace_var sf reg val).
   Proof.
     intros reg val sf tt OLDTYPE NEWTYPE SMALLER WF.
     destruct WF.
@@ -254,13 +259,15 @@ Section ReplaceVar.
   Qed.
 
   Lemma interp_sact_change_vvs:
-    forall vvs1 (VSV1: vvs_smaller_variables vvs1)
-           vvs2 (VSV2: vvs_smaller_variables vvs2) a v
-           (IS: interp_sact (sigma:=sigma) REnv r vvs1 a v)
-           t (WT1: wt_sact (Sigma:=Sigma) R vvs1 a t)
-           (WT2: wt_sact (Sigma:=Sigma) R vvs2 a t)
-           (SMALLER: forall var, reachable_var vvs1 a var -> vvs1 ! var = vvs2 ! var),
-      interp_sact (sigma:=sigma) REnv r vvs2 a v.
+    forall
+      vvs1 (VSV1: vvs_smaller_variables vvs1) vvs2
+      (VSV2: vvs_smaller_variables vvs2) a v
+      (IS: interp_sact (sigma:=sigma) REnv r vvs1 a v) t
+      (WT1: wt_sact (Sigma:=Sigma) R vvs1 a t)
+      (WT2: wt_sact (Sigma:=Sigma) R vvs2 a t)
+      (SMALLER:
+        forall var, reachable_var vvs1 a var -> vvs1 ! var = vvs2 ! var),
+    interp_sact (sigma:=sigma) REnv r vvs2 a v.
   Proof.
     intros.
     eapply interp_eval. 6: apply IS. all: eauto.
@@ -268,37 +275,34 @@ Section ReplaceVar.
   Qed.
 
   Lemma replace_var_interp_rev':
-    forall sf idx v
-           (WFSF: wf_sf sf)
-           (INTERP:
-             forall oldv,
-               interp_sact (sigma:=sigma) REnv r (vars sf) (SVar idx) oldv ->
-               interp_sact (sigma:=sigma) REnv r (vars sf) v oldv
-           )
-           tt (OLDTYPE: wt_sact (Sigma:=Sigma) R (vars sf) (SVar idx) tt),
-        forall oldv,
-          interp_sact (sigma:=sigma) REnv r (vars sf) v oldv ->
-          interp_sact (sigma:=sigma) REnv r (vars sf) (SVar idx) oldv.
+    forall
+      sf idx v (WFSF: wf_sf sf)
+      (INTERP: forall oldv,
+       interp_sact (sigma:=sigma) REnv r (vars sf) (SVar idx) oldv
+       -> interp_sact (sigma:=sigma) REnv r (vars sf) v oldv)
+      tt (OLDTYPE: wt_sact (Sigma:=Sigma) R (vars sf) (SVar idx) tt),
+    forall oldv,
+    interp_sact (sigma:=sigma) REnv r (vars sf) v oldv
+    -> interp_sact (sigma:=sigma) REnv r (vars sf) (SVar idx) oldv.
   Proof.
     intros.
-    edestruct @wt_sact_interp' as (vv & IS & WTV). 6: apply OLDTYPE. all: eauto. apply WFSF. apply WFSF.
+    edestruct @wt_sact_interp' as (vv & IS & WTV). 6: apply OLDTYPE. all: eauto.
+    apply WFSF. apply WFSF.
     eapply wt_sact_valid_vars; eauto. apply vvs_range_max_var.
     eapply INTERP in IS as IS2.
     exploit @interp_sact_determ. apply H. apply IS2. intro; subst. congruence.
   Qed.
 
   Lemma replace_var_interp_rev:
-    forall sf idx v
-           (WFSF: wf_sf sf)
-           (INTERP:
-             forall oldv,
-               interp_sact (sigma:=sigma) REnv r (vars sf) (SVar idx) oldv ->
-               interp_sact (sigma:=sigma) REnv r (vars sf) v oldv
-           )
-           tt (OLDTYPE: wt_sact (Sigma:=Sigma) R (vars sf) (SVar idx) tt),
-        forall oldv,
-          interp_sact (sigma:=sigma) REnv r (vars sf) v oldv <->
-          interp_sact (sigma:=sigma) REnv r (vars sf) (SVar idx) oldv.
+    forall
+      sf idx v (WFSF: wf_sf sf)
+      (INTERP: forall oldv,
+       interp_sact (sigma:=sigma) REnv r (vars sf) (SVar idx) oldv
+       -> interp_sact (sigma:=sigma) REnv r (vars sf) v oldv)
+      tt (OLDTYPE: wt_sact (Sigma:=Sigma) R (vars sf) (SVar idx) tt),
+    forall oldv,
+    interp_sact (sigma:=sigma) REnv r (vars sf) v oldv
+    <-> interp_sact (sigma:=sigma) REnv r (vars sf) (SVar idx) oldv.
   Proof.
     intros.
     split; intros; eauto.
@@ -306,17 +310,16 @@ Section ReplaceVar.
   Qed.
 
   Lemma sf_eq_replace_var:
-    forall sf idx v
-           (WFSF: wf_sf sf)
-           (INTERP:
-             forall oldv,
-               interp_sact (sigma:=sigma) REnv r (vars sf) (SVar idx) oldv ->
-               interp_sact (sigma:=sigma) REnv r (vars sf) v oldv
-           )
-           (SMALLER: forall var, reachable_var (vars sf) v var -> (var < idx)%positive)
-           tt (OLDTYPE: wt_sact (Sigma:=Sigma) R (vars sf) (SVar idx) tt)
-           (NEWTYPE: wt_sact (Sigma:=Sigma) R (vars sf) v tt),
-      sf_eq R Sigma r sigma sf (replace_var sf idx v).
+    forall
+      sf idx v (WFSF: wf_sf sf)
+      (INTERP: forall oldv,
+       interp_sact (sigma:=sigma) REnv r (vars sf) (SVar idx) oldv
+       -> interp_sact (sigma:=sigma) REnv r (vars sf) v oldv)
+      (SMALLER: forall var,
+        reachable_var (vars sf) v var -> (var < idx)%positive)
+      tt (OLDTYPE: wt_sact (Sigma:=Sigma) R (vars sf) (SVar idx) tt)
+      (NEWTYPE: wt_sact (Sigma:=Sigma) R (vars sf) v tt),
+    sf_eq R Sigma r sigma sf (replace_var sf idx v).
   Proof.
     intros.
     split.
@@ -333,14 +336,13 @@ Section ReplaceVar.
 
   Lemma replace_var_interp_cycle_ok':
     forall
-      {reg} {idx} {sf} {v}
-      (WFSF: wf_sf sf)
+      {reg} {idx} {sf} {v} (WFSF: wf_sf sf)
       (INTERP:
         forall oldv,
-          interp_sact (sigma:=sigma) REnv r (vars sf) (SVar idx) oldv ->
-          interp_sact (sigma:=sigma) REnv r (vars sf) v oldv
-      )
-      (SMALLER: forall var, reachable_var (vars sf) v var -> (var < idx)%positive)
+        interp_sact (sigma:=sigma) REnv r (vars sf) (SVar idx) oldv
+        -> interp_sact (sigma:=sigma) REnv r (vars sf) v oldv)
+      (SMALLER:
+        forall var, reachable_var (vars sf) v var -> (var < idx)%positive)
       tt (OLDTYPE: wt_sact (Sigma:=Sigma) R (vars sf) (SVar idx) tt)
       (NEWTYPE: wt_sact (Sigma:=Sigma) R (vars sf) v tt),
     getenv REnv (interp_cycle r sigma sf) reg
@@ -352,27 +354,22 @@ Section ReplaceVar.
     - eapply sf_eq_replace_var; eauto.
   Qed.
 
-  Record var_simpl vvs idx v :=
-    {
-      vs_interp:
-      forall oldv,
-        interp_sact (sigma:=sigma) REnv r vvs (SVar idx) oldv ->
-        interp_sact (sigma:=sigma) REnv r vvs v oldv;
-      vs_smaller:
-      forall var, reachable_var vvs v var -> ((var < idx)%positive);
-      vs_type: type;
-      vs_oldtype: wt_sact (Sigma:=Sigma) R vvs (SVar idx) vs_type;
-      vs_newtype: wt_sact (Sigma:=Sigma) R vvs v vs_type
-    }.
+  Record var_simpl vvs idx v := {
+    vs_interp:
+      forall oldv, interp_sact (sigma:=sigma) REnv r vvs (SVar idx) oldv
+      -> interp_sact (sigma:=sigma) REnv r vvs v oldv;
+    vs_smaller: forall var, reachable_var vvs v var -> ((var < idx)%positive);
+    vs_type: type;
+    vs_oldtype: wt_sact (Sigma:=Sigma) R vvs (SVar idx) vs_type;
+    vs_newtype: wt_sact (Sigma:=Sigma) R vvs v vs_type
+  }.
 
   Lemma wf_sf_replace_var:
-    forall reg val sf
-           (VS: var_simpl (vars sf) reg val),
-      wf_sf sf -> wf_sf (replace_var sf reg val).
+    forall reg val sf (VS: var_simpl (vars sf) reg val),
+    wf_sf sf -> wf_sf (replace_var sf reg val).
   Proof.
     intros reg val sf VS WFSF; inv VS; eapply wf_sf_replace_var'; eauto.
   Qed.
-
 
   Lemma replace_var_interp_cycle_ok:
     forall
@@ -385,5 +382,4 @@ Section ReplaceVar.
     intros. destruct VS.
     eapply replace_var_interp_cycle_ok'; eauto.
   Qed.
-
 End ReplaceVar.
